src/defs/var.lean
@@ -1,16 +1,45 @@
+import util.list
+
 -- any type with infinite values would work
 @[reducible]
 def var: Type := ℕ
 
 @[reducible]
-def cx (t: Type) := list (prod var t)
+def ne_cx_entry {t: Type} (a: prod var t) (b: prod var t): Prop :=
+  a.fst ≠ b.fst
 
-@[reducible]
-def vars {t: Type} (Γ: cx t): list var := list.map prod.fst Γ
+structure cx (t: Type): Type :=
+  (entries: list (prod var t))
+  (nodupkeys: pairwise ne_cx_entry entries)
 
-inductive lookup {t: Type}: cx t -> var -> t -> Prop
-| hd (Γ: cx t) (x: var) (out: t): lookup ((x, out) :: Γ) x out
-| tl (Γ: cx t) (x: var) (out: t) (y: var) (out_y: t):
-    x ≠ y ->
-    lookup Γ x out ->
-    lookup ((y, out_y) :: Γ) x out
+def cx.insert {t: Type} (x: var) (v: t) (Γ: cx t): cx t :=
+begin
+  cases Γ,
+  let p := ne_cx_entry (x, v),
+  let entries' := (x, v) :: list.filter p Γ_entries,
+  let spec := filter_spec p Γ_entries,
+  let spec' := fun a, fun b, (spec a b).right,
+  let nodupkeys' := @pairwise.cons
+    (prod var t) ne_cx_entry (x, v) (list.filter p Γ_entries) spec'
+    (filter_pairwise p Γ_nodupkeys),
+  exact cx.mk entries' nodupkeys',
+end
+
+instance cx_has_insert {t: Type}: has_insert (prod var t) (cx t) :=
+  has_insert.mk (fun a, fun Γ, begin
+    cases a,
+    exact cx.insert a_fst a_snd Γ
+  end)
+
+def cx.lookup {t: Type} (Γ: cx t) (x: var): option t :=
+begin
+  cases Γ,
+  induction Γ_entries,
+  exact none,
+  cases Γ_entries_hd,
+  exact (if x = Γ_entries_hd_fst then
+    some Γ_entries_hd_snd
+  else
+    Γ_entries_ih (pairwise_inversion Γ_nodupkeys)
+  ),
+end
