src/util/list.lean
@@ -1,0 +1,87 @@
+inductive pairwise {t: Type} (r: t -> t -> Prop): list t → Prop
+| nil: pairwise []
+| cons {x: t} {xs: list t}: (∀ y ∈ xs, r x y) -> pairwise xs -> pairwise (x :: xs)
+
+-- don't know why this is necessary
+theorem pairwise_inversion {t: Type} {r: t -> t -> Prop} {x: t} {xs: list t}:
+  pairwise r (x :: xs) -> pairwise r xs :=
+begin
+  intro h,
+  cases h,
+  exact h_a_1,
+end
+
+theorem filter_spec {t: Type} (p: t -> Prop) (xs: list t)
+  [decidable_pred p]:
+  ∀ x ∈ list.filter p xs, (x ∈ xs) ∧ (p x) :=
+begin
+  intros x h,
+  induction xs,
+  simp [list.filter] at h,
+  exfalso,
+  exact h,
+  simp [list.filter] at h,
+  -- maybe could use decidable_pred p here somehow to have a justification for
+  -- using excluded middle?
+  cases classical.em (p xs_hd),
+  simp [h_1] at h,
+  cases h,
+  rw h,
+  split,
+  simp,
+  exact h_1,
+  cases xs_ih h,
+  split,
+  simp,
+  right,
+  exact left,
+  exact right,
+  simp [h_1] at h,
+  cases xs_ih h,
+  split,
+  simp,
+  right,
+  exact left,
+  exact right,
+end
+
+theorem filter_pairwise {t: Type} {r: t -> t -> Prop} {xs: list t}
+  (p: t -> Prop)
+  [decidable_pred p]:
+  pairwise r xs ->
+  pairwise r (list.filter p xs) :=
+begin
+  intro h,
+  induction h,
+  simp [list.filter],
+  exact pairwise.nil r,
+  simp [list.filter],
+  cases classical.em (p h_x),
+  simp [h],
+  let f: ∀ (y: t), y ∈ list.filter p h_xs -> r h_x y := fun a, fun b,
+    h_a a (filter_spec p h_xs a b).left,
+  exact pairwise.cons f h_ih,
+  simp [h],
+  exact h_ih,
+end
+
+theorem append_nil_both
+  {t: Type} (xs ys: list t): xs ++ ys = [] ↔ xs = [] ∧ ys = [] :=
+begin
+  split,
+  intro h,
+  induction xs,
+  induction ys,
+  split,
+  refl,
+  refl,
+  split,
+  refl,
+  cases h,
+  cases h,
+  intro h,
+  cases h,
+  rw h_left,
+  rw h_right,
+  simp [list.append],
+end
